wip

CoqOfRust/stack/core/option.v
@@ -42,6 +42,7 @@ Module Impl_core_option_Option_T.
     eapply Run.CallPrimitiveStateRead. {
       apply Stack.HasReadWith.Immediate.
     }
+    fold @LowM.let_.
     cbn.
     apply Run.CallGetSubPointer with (H_read := H_self_pointer).
     destruct self as [self|]; cbn.
@@ -62,4 +63,145 @@ Module Impl_core_option_Option_T.
       apply Run.Pure.
     }
   Qed.
+
+  Definition is_none {A : Set} (self : Self A) : bool :=
+    negb (is_some self).
+
+  Lemma run_is_none {A : Set} (A_ty : Ty.t) (A_to_value : A -> Value.t)
+      (self_pointer : Pointer.t Value.t) (self : Self A)
+      (stack : Stack.t) :
+    let self_value : Value.t := to_value A_to_value self in
+    Stack.HasReadWith.t stack self_value self_pointer ->
+    {{ stack |
+      CoqOfRust.core.option.option.Impl_core_option_Option_T.is_none
+        A_ty [] [] [Value.Pointer self_pointer] ⇓
+      inl (Value.Bool (is_none self))
+    | stack }}.
+  Proof.
+    intros * H_self_pointer.
+    unfold option.option.Impl_core_option_Option_T.is_none.
+    eapply Run.CallPrimitiveStateAlloc. {
+      apply Stack.HasAllocWith.Immediate.
+    }
+    eapply Run.CallPrimitiveGetAssociatedFunction. {
+      apply option.option.Impl_core_option_Option_T.AssociatedFunction_is_some.
+    }
+    fold @LowM.let_.
+    eapply Run.CallPrimitiveStateRead. {
+      apply Stack.HasReadWith.Immediate.
+    }
+    fold @LowM.let_.
+    eapply Run.CallClosure. {
+      apply run_is_some with (A_to_value := A_to_value).
+      apply H_self_pointer.
+    }
+    apply Run.Pure.
+  Qed.
+
+  Definition as_ref {A : Set} (self : Self A) : Self A :=
+    self.
+
+  Lemma run_as_ref {A : Set} (A_ty : Ty.t) (A_to_value : A -> Value.t)
+      (self_pointer : Pointer.t Value.t) (self : Self A)
+      (stack : Stack.t) :
+    let self_value : Value.t := to_value A_to_value self in
+    Stack.HasReadWith.t stack self_value self_pointer ->
+    {{ stack |
+      CoqOfRust.core.option.option.Impl_core_option_Option_T.as_ref
+        A_ty [] [] [Value.Pointer self_pointer] ⇓
+      inl self_value
+    | stack }}.
+  Proof.
+    intros * H_self_pointer.
+    unfold option.option.Impl_core_option_Option_T.as_ref.
+    eapply Run.CallPrimitiveStateAlloc. {
+      apply Stack.HasAllocWith.Immediate.
+    }
+    eapply Run.CallPrimitiveStateRead. {
+      apply Stack.HasReadWith.Immediate.
+    }
+    fold @LowM.let_.
+    apply Run.CallGetSubPointer with (H_read := H_self_pointer).
+    fold @LowM.let_.
+    destruct self as [self|]; cbn.
+    { eapply Run.CallPrimitiveStateAlloc. {
+        apply Stack.HasAllocWith.Immediate.
+      }
+      eapply Run.CallPrimitiveStateRead. {
+        apply Stack.HasReadWith.Immediate.
+      }
+      eapply Run.CallPrimitiveStateAlloc. {
+        apply Stack.HasAllocWith.Immediate.
+      }
+      eapply Run.CallPrimitiveStateRead. {
+        apply Stack.HasReadWith.Immediate.
+      }
+      admit.
+    }
+    { eapply Run.CallPrimitiveStateRead. {
+        apply H_self_pointer.
+      }
+      cbn.
+      eapply Run.CallPrimitiveStateAlloc. {
+        apply Stack.HasAllocWith.Immediate.
+      }
+      eapply Run.CallPrimitiveStateRead. {
+        apply Stack.HasReadWith.Immediate.
+      }
+      apply Run.Pure.
+    }
+  Admitted.
+
+  Axiom expect_failed : forall {A : Set}, string -> A.
+
+  (*
+      pub const fn expect(self, msg: &str) -> T {
+          match self {
+              Some(val) => val,
+              None => expect_failed(msg),
+          }
+      }
+  *)
+  Definition expect {A : Set} (self : Self A) (msg : string) : A :=
+    match self with
+    | Some val => val
+    | None => expect_failed msg
+    end.
+
+  Lemma run_expect {A : Set} (A_ty : Ty.t) (A_to_value : A -> Value.t)
+      (self : Self A) (msg : string)
+      (stack : Stack.t) :
+    let self_value : Value.t := to_value A_to_value self in
+    {{ stack |
+      CoqOfRust.core.option.option.Impl_core_option_Option_T.expect
+        A_ty [] [] [self_value; Value.String msg] ⇓
+      inl (A_to_value (expect self msg))
+    | stack }}.
+  Proof.
+    intros.
+    unfold option.option.Impl_core_option_Option_T.expect.
+    eapply Run.CallPrimitiveStateAlloc. {
+      apply Stack.HasAllocWith.Immediate.
+    }
+    eapply Run.CallPrimitiveStateAlloc. {
+      apply Stack.HasAllocWith.Immediate.
+    }
+    destruct self as [self|]; cbn.
+    { eapply Run.CallGetSubPointer.
+      cbn.
+        apply Stack.HasAllocWith.Immediate.
+      }
+      eapply Run.CallPrimitiveStateRead. {
+        apply Stack.HasReadWith.Immediate.
+      }
+      apply Run.Pure.
+    }
+    { eapply Run.CallPrimitiveStateAlloc. {
+        apply Stack.HasAllocWith.Immediate.
+      }
+      eapply Run.CallPrimitiveStateRead. {
+        apply Stack.HasReadWith.Immediate.
+      }
+      apply Run.Pure.
+    }
 End Impl_core_option_Option_T.
