CoqOfRust/move_sui/simulations/move_bytecode_verifier/type_safety.v
@@ -1,6 +1,5 @@
 Require Import CoqOfRust.CoqOfRust.
 Require Import CoqOfRust.simulations.M.
-Require Import CoqOfRust.lib.lib.
 
 Import simulations.M.Notations.
 
